Refactor for rename from "gokv/urpc/rpc" to "gokv/urpc"

etc/update-goose.py
@@ -229,7 +229,7 @@ def main():
         run_goose(distributed_dir, ".", "./grove_common")
 
     if gokv_dir is not None:
-        pkgs = ["urpc/rpc", "memkv", "connman", "paxi/single", "bank",
+        pkgs = ["urpc", "memkv", "connman", "paxi/single", "bank",
                 "lockservice", "pb", "pb/controller", "ctrexample/client",
                 "ctrexample/server", "fencing/ctr", "fencing/config",
                 "fencing/frontend", "fencing/client"]
