external/Goose/github_com/mit_pdos/gokv/fencing/config.v
@@ -2,7 +2,7 @@
 From Perennial.goose_lang Require Import prelude.
 From Perennial.goose_lang Require Import ffi.grove_prelude.
 
-From Goose Require github_com.mit_pdos.gokv.urpc.rpc.
+From Goose Require github_com.mit_pdos.gokv.urpc.
 From Goose Require github_com.tchajed.marshal.
 
 (* client.go *)
@@ -24,7 +24,7 @@ Definition Clerk__HeartbeatThread: val :=
     (for: (λ: <>, #true); (λ: <>, Skip) := λ: <>,
       let: "reply_ptr" := ref (zero_val (slice.T byteT)) in
       grove_ffi.Sleep (("TIMEOUT_MS" * "MILLION") `quot` #3);;
-      let: "err" := rpc.RPCClient__Call (struct.loadF Clerk "cl" "ck") RPC_LOCK "args" "reply_ptr" #100 in
+      let: "err" := urpc.Client__Call (struct.loadF Clerk "cl" "ck") RPC_LOCK "args" "reply_ptr" #100 in
       (if: ("err" ≠ #0) || (slice.len (![slice.T byteT] "reply_ptr") ≠ #0)
       then Break
       else Continue));;
@@ -35,7 +35,7 @@ Definition Clerk__Lock: val :=
     let: "enc" := marshal.NewEnc #8 in
     marshal.Enc__PutInt "enc" "newFrontend";;
     let: "reply_ptr" := ref (zero_val (slice.T byteT)) in
-    let: "err" := rpc.RPCClient__Call (struct.loadF Clerk "cl" "ck") RPC_LOCK (marshal.Enc__Finish "enc") "reply_ptr" #100 in
+    let: "err" := urpc.Client__Call (struct.loadF Clerk "cl" "ck") RPC_LOCK (marshal.Enc__Finish "enc") "reply_ptr" #100 in
     (if: "err" ≠ #0
     then
       (* log.Println("config: client failed to run RPC on config server") *)
@@ -47,7 +47,7 @@ Definition Clerk__Lock: val :=
 Definition Clerk__Get: val :=
   rec: "Clerk__Get" "ck" :=
     let: "reply_ptr" := ref (zero_val (slice.T byteT)) in
-    let: "err" := rpc.RPCClient__Call (struct.loadF Clerk "cl" "ck") RPC_LOCK (NewSlice byteT #0) "reply_ptr" #100 in
+    let: "err" := urpc.Client__Call (struct.loadF Clerk "cl" "ck") RPC_LOCK (NewSlice byteT #0) "reply_ptr" #100 in
     (if: "err" ≠ #0
     then
       (* log.Println("config: client failed to run RPC on config server") *)
@@ -59,7 +59,7 @@ Definition Clerk__Get: val :=
 Definition MakeClerk: val :=
   rec: "MakeClerk" "host" :=
     let: "ck" := struct.alloc Clerk (zero_val (struct.t Clerk)) in
-    struct.storeF Clerk "cl" "ck" (rpc.MakeRPCClient "host");;
+    struct.storeF Clerk "cl" "ck" (urpc.MakeClient "host");;
     "ck".
 
 (* server.go *)
@@ -169,6 +169,6 @@ Definition StartServer: val :=
       "reply" <-[slice.T byteT] marshal.Enc__Finish "enc";;
       #()
       );;
-    let: "r" := rpc.MakeRPCServer "handlers" in
-    rpc.RPCServer__Serve "r" "me" #1;;
+    let: "r" := urpc.MakeServer "handlers" in
+    urpc.Server__Serve "r" "me";;
     #().
