src/program_proof/fencing/ctr_proof.v
@@ -2,53 +2,106 @@ From Perennial.program_proof Require Import grove_prelude.
 From Goose.github_com.mit_pdos.gokv.fencing Require Import ctr.
 From Perennial.program_proof Require Import grove_prelude.
 From Perennial.program_proof.memkv Require Export rpc_lib rpc_proof rpc_spec.
+From iris.algebra Require Import cmra.
+From iris.base_logic Require Import mono_nat.
+
+From Perennial.program_proof.fencing Require Export map.
 
 Section ctr_definitions.
+
 Context `{!gooseGlobalGS Σ}.
 Context `{!heapGS Σ}.
 
 Record ctr_names :=
-  {}.
+{
+  epoch_gn : gname ;
+  epoch_token_gn : gname ;
+  val_gn : gname ;
+}.
 
-Definition own_epoch (e:u64) (q:Qp): iProp Σ.
-Admitted.
+Implicit Type γ : ctr_names.
 
-Definition own_val (e:u64) (v:option u64) (q:Qp): iProp Σ.
-Admitted.
+Context `{!mono_natG Σ}.
+Context `{!mapG Σ u64 u64}.
+Context `{!mapG Σ u64 unit}.
 
-Global Instance own_epoch_timeless e q : Timeless (own_epoch e q).
-Admitted.
+Definition own_latest_epoch γ (e:u64) (q:Qp) : iProp Σ :=
+  mono_nat_auth_own γ.(epoch_gn) q (int.nat e).
 
-Global Instance own_val_timeless e v q : Timeless (own_val e v q).
-Admitted.
+Definition is_latest_epoch_lb γ (e:u64) : iProp Σ :=
+  mono_nat_lb_own γ.(epoch_gn) (int.nat e).
+
+Definition own_unused_epoch γ (e:u64) : iProp Σ :=
+  e ⤳[γ.(epoch_token_gn)] ().
+
+Definition own_val γ (e:u64) (v:u64) (q:Qp): iProp Σ :=
+  e ⤳[γ.(val_gn)]{# q } v.
 
 Definition own_Clerk (ck:loc) : iProp Σ.
 Admitted.
 
-(* FIXME: In the case where oldv = None, we need to ensure that v is the last
-   value from latestEpoch. In fact, we can just give the client that old epoch
-   points-to half, because the server doesn't want it anymore. *)
-Lemma wp_Clerk__Get {Eo Ei Ei2:coPset} ck (e:u64) :
+(* NOTE: consider lt_eq_lt_dec: ∀ n m : nat, {n < m} + {n = m} + {m < n} *)
+Lemma wp_Clerk__Get γ ck (e:u64) :
   ∀ Φ,
   own_Clerk ck -∗
-  (|={Eo,Ei}=> ∃ latestEpoch, own_epoch latestEpoch (1/2)%Qp ∗
-    (*(⌜int.Z latestEpoch > int.Z e⌝ → epoch_ptsto latestEpoch ={Ei, Eo}=∗ Φ #EStale) ∗*) (* XXX: program exits in this case *)
-    (⌜int.Z latestEpoch ≤ int.Z e⌝ → own_epoch e (1/2)%Qp ={Ei}=∗ (* XXX: one inner mask is probably enough, thhough we could have multiple invariants *)
-     (∃ oldv, own_val e oldv (1/2)%Qp ∗ (∀ v, ⌜is_Some oldv → oldv = Some v⌝ →
-                                               own_val e (Some v) (1/2)%Qp ={Ei2,Eo}=∗
-                                                              (own_Clerk ck -∗ Φ #v))))) -∗
-    WP Clerk__Get #ck #e @ Eo {{ Φ }}.
+  (|={⊤,∅}=> ∃ latestEpoch, own_latest_epoch γ latestEpoch (1/2)%Qp ∗
+    if decide (int.Z latestEpoch < int.Z e)%Z then
+      own_unused_epoch γ e ∗
+                            (∀ v, own_val γ e v (1/2)%Qp ∗
+                                           own_val γ latestEpoch v (1/2)%Qp ∗
+                                           own_latest_epoch γ e (1/2)%Qp
+                                           ={∅,⊤}=∗ (own_Clerk ck -∗ Φ #v))
+   else if decide (latestEpoch = e) then
+   ∃ v, own_val γ e v (1/2)%Qp ∗
+    (own_val γ e v (1/2)%Qp ∗ own_latest_epoch γ e (1/2)%Qp ={∅,⊤}=∗ (own_Clerk ck -∗ Φ #v))
+   else
+     True) -∗
+    WP Clerk__Get #ck #e {{ Φ }}.
 Proof.
 Admitted.
 
-Lemma wp_Clerk__Put {Eo Ei Ei2:coPset} ck (k e v:u64) :
+Lemma wp_Clerk__Put γ ck (e v:u64) :
   ∀ Φ,
   own_Clerk ck -∗
-  (|={Eo,Ei}=> ∃ latestEpoch, own_epoch latestEpoch (1/2)%Qp ∗
-    (*(⌜int.Z latestEpoch > int.Z e⌝ → epoch_ptsto latestEpoch ={Ei, Eo}=∗ Φ #EStale) ∗*) (* XXX: program exits in this case *)
-    (⌜int.Z latestEpoch ≤ int.Z e⌝ → own_epoch e (1/2)%Qp ={Ei}=∗ (* XXX: one inner mask is probably enough, thhough we could have multiple invariants *)
-     (∃ oldv, own_val e oldv (1/2)%Qp ∗ (own_val e (Some v) (1/2)%Qp ={Ei2,Eo}=∗ (own_Clerk ck -∗ Φ #v))))) -∗
-    WP Clerk__Get #ck #e @ Eo {{ Φ }}.
+  (|={⊤,∅}=> ∃ latestEpoch, own_latest_epoch γ latestEpoch (1/2)%Qp ∗
+    if decide (int.Z latestEpoch < int.Z e)%Z then
+      own_unused_epoch γ e ∗
+                            (∀ oldv, own_val γ e v (1/2)%Qp ∗
+                                           own_val γ latestEpoch oldv (1/2)%Qp ∗
+                                           own_latest_epoch γ e (1/2)%Qp
+                                           ={∅,⊤}=∗ (own_Clerk ck -∗ Φ #v))
+   else if decide (latestEpoch = e) then
+   ∃ oldv, own_val γ e oldv (1/2)%Qp ∗
+    (own_val γ e v (1/2)%Qp ∗ own_latest_epoch γ e (1/2)%Qp ={∅,⊤}=∗ (own_Clerk ck -∗ Φ #v))
+   else
+     True) -∗
+    WP Clerk__Put #ck #e #v {{ Φ }}.
+Proof.
+Admitted.
+
+Lemma wp_Clerk__Get' γ ck (e:u64) :
+  ∀ Φ,
+  own_Clerk ck -∗
+  (|={⊤,∅}=> ∃ latestEpoch, own_latest_epoch γ latestEpoch (1/2)%Qp ∗
+   ∃ v, own_val γ e v (1/2)%Qp ∗
+  ( own_val γ e v (1/2)%Qp ∗
+    own_latest_epoch γ e (1/2)%Qp ∗
+    if decide (int.Z latestEpoch < int.Z e)%Z then
+      own_val γ latestEpoch v (1/2)%Qp
+    else ⌜latestEpoch = e⌝
+    ={∅,⊤}=∗ (own_Clerk ck -∗ Φ #v))) -∗
+    WP Clerk__Get #ck #e {{ Φ }}.
+Proof.
+Admitted.
+
+Lemma wp_Clerk__Get'' γ ck (e:u64) :
+  ∀ Φ,
+  own_Clerk ck -∗
+  (|={⊤,∅}=>
+     (own_unused_epoch γ e ∗ (∃ v, own_val γ e v (1/2)%Qp
+           ={∅,⊤}=∗ (own_Clerk ck -∗ Φ #v))) ∨
+     (∃ v, own_val γ e v (1/2) ∗ (own_val γ e v (1/2) ={∅,⊤}=∗ (own_Clerk ck -∗ Φ #v)))) -∗
+    WP Clerk__Get #ck #e {{ Φ }}.
 Proof.
 Admitted.
 
