src/program_proof/fencing/frontend_proof.v
@@ -23,20 +23,16 @@ Admitted.
 Definition is_mepoch_lb (e:u64) : iProp Σ.
 Admitted.
 
-Definition own_mepoch (e:u64) : iProp Σ.
-Admitted.
+Context `{!inG Σ epochR}.
+Context `{!inG Σ valR}.
 
-Global Instance own_mepoch_timeless e : Timeless (own_mepoch e).
-Admitted.
-
-Definition frontend_inv_def: iProp Σ :=
+Definition frontend_inv_def γ: iProp Σ :=
   ∃ (latestEpoch v:u64),
-  "HlatestEpoch" ∷ own_epoch latestEpoch q2 ∗
-  "HlatestMEpoch" ∷ own_mepoch latestEpoch ∗
-  "Hval" ∷ own_val latestEpoch (Some v) q4 ∗
+  "HlatestEpoch" ∷ own_latest_epoch γ latestEpoch q2 ∗
+  "Hval" ∷ own_val γ latestEpoch (Some v) q4 ∗
   "Hkv" ∷ kv_ptsto k0 v.
 
-Definition own_Server (s:loc) (epoch:u64) : iProp Σ :=
+Definition own_FrontendServer (s:loc) γ (epoch:u64) : iProp Σ :=
   ∃ (ck1 ck2:loc),
   "#Hepoch" ∷ readonly (s ↦[frontend.Server :: "epoch"] #epoch) ∗
   "Hck1" ∷ s ↦[frontend.Server :: "ck1"] #ck1 ∗
@@ -44,24 +40,23 @@ Definition own_Server (s:loc) (epoch:u64) : iProp Σ :=
   "Hck1_own" ∷ own_Clerk ck1 ∗
   "Hck2_own" ∷ own_Clerk ck2 ∗
 
-  "Hghost1" ∷ (∃ ov, own_val epoch ov q2 ∨ is_mepoch_lb epoch ∗ own_val epoch ov q4) ∗
+  "Hghost1" ∷ (own_unused_epoch γ epoch ∨ (∃ v, is_mepoch_lb epoch ∗ own_val γ epoch (Some v) q4)).
   (* TODO: add second value *)
-  "_" ∷ True.
 
 Definition frontendN := nroot .@ "frontend".
 
-Definition is_Server s : iProp Σ :=
+Definition is_Server s γ : iProp Σ :=
   ∃ mu,
   "Hmu" ∷ readonly (s ↦[frontend.Server :: "mu"] mu) ∗
-  "HmuInv" ∷ is_lock frontendN mu (∃ epoch, own_Server s epoch)
+  "HmuInv" ∷ is_lock frontendN mu (∃ epoch, own_FrontendServer s γ epoch)
 .
-Definition frontend_inv : iProp Σ :=
-  inv frontendN (frontend_inv_def).
+Definition frontend_inv γ : iProp Σ :=
+  inv frontendN (frontend_inv_def γ).
 
-Lemma wp_FetchAndIncrement (s:loc) (key:u64) :
+Lemma wp_FetchAndIncrement (s:loc) γ (key:u64) :
   key = 0 ∨ key = 1 →
-  is_Server s -∗
-  frontend_inv -∗
+  is_Server s γ -∗
+  frontend_inv γ -∗
   {{{
         True
   }}}
@@ -93,7 +88,24 @@ Proof.
     iNamed "Hown".
     iModIntro.
     iExists _; iFrame "HlatestEpoch".
-    iIntros "%Hfresh HlatestEpoch".
+    destruct (decide (int.Z latestEpoch < int.Z epoch)) as [Hineq|Hineq].
+    { (* case: epoch number is new *)
+      admit.
+    }
+    { (* case: ctr server already knows about latest epoch number *)
+      destruct (decide (latestEpoch = epoch)) as [Heq|Hbad]; last done.
+      rewrite Heq.
+      iDestruct "Hghost1" as "[Hbad|Hghost1]".
+      { (* non-matching case, contradictory*)
+        iExFalso.
+        admit.
+      }
+      {
+        iDestruct "Hghost1" as (v') "Hghost1".
+        (* TODO: lemma to combine fractions of own_val *)
+      }
+    }
+
     iModIntro.
     iAssert (∃ oldv, own_val epoch oldv (1/2))%I with "[Hghost1]" as (?) "HH".
     {
